bfffff

theories/dyn_lang/labels.v
@@ -1,65 +1,38 @@
 From main Require Import imports dyn_lang.definition.
 
-Definition LabelRel := relation label.
-
-Definition le_permissive : relation LabelRel :=
-  fun L1 L2 => (∀ ℓ ℓ', L1 ℓ ℓ' → L2 ℓ ℓ') .
-
-Notation "L1 ≤ L2" := (le_permissive L1 L2).
-
-Instance le_permissive_trans : Transitive le_permissive.
-Proof. intros R1 R2 R3 H12 H23 ℓ ℓ' Hℓℓ'. by apply H23, H12. Qed.
-
-Lemma le_permissive_trans' Δ1 Δ2 Δ3 :
-  le_permissive Δ2 Δ3 → le_permissive Δ1 Δ2 → le_permissive Δ1 Δ3.
-Proof. intros. by eapply transitivity. Qed.
-
-Definition PermitNone : LabelRel := fun _ _ => False.
-(* Notation "∅" := (PermitNone). *)
-
-Definition PermitAll : LabelRel := fun _ _ => False.
-(* Notation "#" := (PermitAll). *)
-
-Definition unary_conj (L : label → Prop) : LabelRel :=
-  fun ℓ ℓ' => L ℓ ∧ L ℓ'.
-
-Lemma le_perm_unary_conj L L' (H : ∀ ℓ, L ℓ → L' ℓ) :
-  le_permissive (unary_conj L) (unary_conj L').
-Proof. intros ℓ ℓ' H'. destruct H'. split; by eapply H. Qed.
-
-Fixpoint getLabels (e : expr) : listset label :=
+Fixpoint labels_expr (e : expr) : listset label :=
     match e with
     | Lit b => ∅
     | Seq ℓ e1 e2 =>
-        {[ ℓ ]} ∪ getLabels e1 ∪ getLabels e2
+        {[ ℓ ]} ∪ labels_expr e1 ∪ labels_expr e2
     | If ℓ e0 e1 e2 =>
-        {[ ℓ ]} ∪ getLabels e0 ∪ getLabels e1 ∪ getLabels e2
+        {[ ℓ ]} ∪ labels_expr e0 ∪ labels_expr e1 ∪ labels_expr e2
     | BinOp ℓ binop e1 e2 =>
-        {[ ℓ ]} ∪ getLabels e1 ∪ getLabels e2
+        {[ ℓ ]} ∪ labels_expr e1 ∪ labels_expr e2
     | Var v => ∅
     | Lam e =>
-        getLabels e
+        labels_expr e
     | App ℓ e1 e2 =>
-        {[ ℓ ]} ∪ getLabels e1 ∪ getLabels e2
+        {[ ℓ ]} ∪ labels_expr e1 ∪ labels_expr e2
     | InjL e =>
-        getLabels e
+        labels_expr e
     | InjR e =>
-        getLabels e
+        labels_expr e
     | Case ℓ e0 e1 e2 =>
-        {[ ℓ ]} ∪ getLabels e0 ∪ getLabels e1 ∪ getLabels e2
+        {[ ℓ ]} ∪ labels_expr e0 ∪ labels_expr e1 ∪ labels_expr e2
     | Fst ℓ e =>
-        {[ ℓ ]} ∪ getLabels e
+        {[ ℓ ]} ∪ labels_expr e
     | Snd ℓ e =>
-        {[ ℓ ]} ∪ getLabels e
+        {[ ℓ ]} ∪ labels_expr e
     | Pair e1 e2 =>
-        getLabels e1 ∪ getLabels e2
+        labels_expr e1 ∪ labels_expr e2
     | Error ℓ =>
         {[ ℓ ]}
     end.
 
-Definition occursIn (e : expr) : label → Prop := fun ℓ => ℓ ∈ getLabels e.
+(* Definition occursIn (e : expr) : label → Prop := fun ℓ => ℓ ∈ (labels_expr e). *)
 
-Definition Lbls (e : expr) : LabelRel :=
-  unary_conj (occursIn e).
+Definition InDynExpr (e : expr) : LabelRel :=
+  unary_conj (fun ℓ => ℓ ∈ (labels_expr e)).
 
 (* Notation "Δ e" := (Diagonal e) (at level 0). *)
