theories/grad_lang/typing.v
@@ -38,7 +38,83 @@ Inductive typed (Γ : list type) : expr → type → Prop :=
     Γ ⊢ e0 : Bin Sum τ1 τ2 → τ1 :: Γ ⊢ e1 : τ3 → τ2 :: Γ ⊢ e2 : τ3 →
     Γ ⊢ Case e0 e1 e2 : τ3
  (* assert! *)
- | Ascribe_typed ℓ τ1 τ2 e :
+ | Ascribe_typed ℓ τ1 τ2 (H : consistency τ1 τ2) e :
     Γ ⊢ e : τ1 → Γ ⊢ Ascribe ℓ τ1 τ2 e : τ2
 
 where "Γ ⊢ e : τ" := (typed Γ e τ).
+
+From main.grad_lang Require Import contexts.
+
+Inductive typed_ctx_item :
+    ctx_item → list type → type → list type → type → Prop :=
+  | TP_CTX_Lam Γ τ τ' :
+    typed_ctx_item CTX_Lam (τ :: Γ) τ' Γ (Bin Arrow τ τ')
+  | TP_CTX_AppL Γ e2 τ τ' :
+    typed Γ e2 τ →
+    typed_ctx_item (CTX_AppL e2) Γ (Bin Arrow τ τ') Γ τ'
+  | TP_CTX_AppR Γ e1 τ τ' :
+    typed Γ e1 (Bin Arrow τ τ') →
+    typed_ctx_item (CTX_AppR e1) Γ τ Γ τ'
+  | TP_CTX_PairL Γ e2 τ τ' :
+    typed Γ e2 τ' →
+    typed_ctx_item (CTX_PairL e2) Γ τ Γ (Bin Product τ τ')
+  | TP_CTX_PairR Γ e1 τ τ' :
+    typed Γ e1 τ →
+    typed_ctx_item (CTX_PairR e1) Γ τ' Γ (Bin Product τ τ')
+  | TP_CTX_Fst Γ τ τ' :
+    typed_ctx_item CTX_Fst Γ (Bin Product τ τ') Γ τ
+  | TP_CTX_Snd Γ τ τ' :
+    typed_ctx_item CTX_Snd Γ (Bin Product τ τ') Γ τ'
+  | TP_CTX_InjL Γ τ τ' :
+    typed_ctx_item CTX_InjL Γ τ Γ (Bin Sum τ τ')
+  | TP_CTX_InjR Γ τ τ' :
+    typed_ctx_item CTX_InjR Γ τ' Γ (Bin Sum τ τ')
+  | TP_CTX_CaseL Γ e1 e2 τ1 τ2 τ' :
+    typed (τ1 :: Γ) e1 τ' → typed (τ2 :: Γ) e2 τ' →
+    typed_ctx_item (CTX_CaseL e1 e2) Γ (Bin Sum τ1 τ2) Γ τ'
+  | TP_CTX_CaseM Γ e0 e2 τ1 τ2 τ' :
+    typed Γ e0 (Bin Sum τ1 τ2) → typed (τ2 :: Γ) e2 τ' →
+    typed_ctx_item (CTX_CaseM e0 e2) (τ1 :: Γ) τ' Γ τ'
+  | TP_CTX_CaseR Γ e0 e1 τ1 τ2 τ' :
+    typed Γ e0 (Bin Sum τ1 τ2) → typed (τ1 :: Γ) e1 τ' →
+    typed_ctx_item (CTX_CaseR e0 e1) (τ2 :: Γ) τ' Γ τ'
+  | TP_CTX_BinOpL op Γ e2 :
+    typed Γ e2 (Base Int) →
+    typed_ctx_item (CTX_BinOpL op e2) Γ (Base Int) Γ (binop_res_type op)
+  | TP_CTX_BinOpR op e1 Γ :
+    typed Γ e1 (Base Int) →
+    typed_ctx_item (CTX_BinOpR op e1) Γ (Base Int) Γ (binop_res_type op)
+  | TP_CTX_IfL Γ e1 e2 τ :
+    typed Γ e1 τ → typed Γ e2 τ →
+    typed_ctx_item (CTX_IfL e1 e2) Γ ((Base Bool)) Γ τ
+  | TP_CTX_IfM Γ e0 e2 τ :
+    typed Γ e0 ((Base Bool)) → typed Γ e2 τ →
+    typed_ctx_item (CTX_IfM e0 e2) Γ τ Γ τ
+  | TP_CTX_IfR Γ e0 e1 τ :
+    typed Γ e0 ((Base Bool)) → typed Γ e1 τ →
+    typed_ctx_item (CTX_IfR e0 e1) Γ τ Γ τ
+  | TP_CTX_SeqL Γ e2 τ :
+    typed Γ e2 τ →
+    typed_ctx_item (CTX_SeqL e2) Γ (Base Unit) Γ τ
+  | TP_CTX_SeqR Γ e1 τ :
+    typed Γ e1 (Base Unit) →
+    typed_ctx_item (CTX_SeqR e1) Γ τ Γ τ
+  | TP_CTX_Ascribe Γ ℓ τ1 τ2 (H : consistency τ1 τ2) :
+    typed_ctx_item (CTX_Ascribe ℓ τ1 τ2) Γ τ1 Γ τ2.
+
+Lemma typed_ctx_item_typed k Γ τ Γ' τ' e :
+  typed Γ e τ → typed_ctx_item k Γ τ Γ' τ' →
+  typed Γ' (fill_ctx_item k e) τ'.
+Proof. induction 2; simpl; eauto using typed. Qed.
+
+Inductive typed_ctx : ctx → list type → type → list type → type → Prop :=
+  | TPCTX_nil Γ τ :
+    typed_ctx nil Γ τ Γ τ
+  | TPCTX_cons Γ1 τ1 Γ2 τ2 Γ3 τ3 Ci C :
+    typed_ctx_item Ci Γ2 τ2 Γ3 τ3 →
+    typed_ctx C Γ1 τ1 Γ2 τ2 →
+    typed_ctx (Ci :: C) Γ1 τ1 Γ3 τ3.
+
+Lemma typed_ctx_typed K Γ τ Γ' τ' e :
+  typed Γ e τ → typed_ctx K Γ τ Γ' τ' → typed Γ' (fill_ctx K e) τ'.
+Proof. induction 2; simpl; eauto using typed_ctx_item_typed. Qed.
