theories/prelude/labels.v
@@ -4,3 +4,45 @@ From stdpp Require Import listset.
 Inductive label : Set := Lbl (ℓ : Z).
 
 Class NeverOccurs (ℓ : label) : Type.
+
+Definition LabelRel := relation label.
+
+Definition le_permissive : relation LabelRel :=
+  fun L1 L2 => (∀ ℓ ℓ', L1 ℓ ℓ' → L2 ℓ ℓ') .
+
+Definition equiv_LabelRel (L L' : LabelRel) :=
+  ∀ ℓ ℓ', L ℓ ℓ' <-> L' ℓ ℓ' .
+
+Notation "L1 ≤ L2" := (le_permissive L1 L2).
+
+Instance le_permissive_trans : Transitive le_permissive.
+Proof. intros R1 R2 R3 H12 H23 ℓ ℓ' Hℓℓ'. by apply H23, H12. Qed.
+
+Lemma le_permissive_trans' Δ1 Δ2 Δ3 :
+  le_permissive Δ2 Δ3 → le_permissive Δ1 Δ2 → le_permissive Δ1 Δ3.
+Proof. intros. by eapply transitivity. Qed.
+
+Definition PermitNone : LabelRel := fun _ _ => False.
+(* Notation "∅" := (PermitNone). *)
+
+Definition PermitAll : LabelRel := fun _ _ => False.
+(* Notation "#" := (PermitAll). *)
+
+Definition disj (L1 L2 : LabelRel) : LabelRel :=
+  fun ℓ ℓ' => L1 ℓ ℓ' ∨ L2 ℓ ℓ'.
+
+Definition unary_conj (L : label → Prop) : LabelRel :=
+  fun ℓ ℓ' => L ℓ ∧ L ℓ'.
+
+Lemma le_perm_unary_conj L L' (H : ∀ ℓ, L ℓ → L' ℓ) :
+  le_permissive (unary_conj L) (unary_conj L').
+Proof. intros ℓ ℓ' H'. destruct H'. split; by eapply H. Qed.
+
+Definition elemhood (ℓs : listset label) : label → Prop :=
+  fun ℓ => ℓ ∈ ℓs.
+
+(* Lemma disj_union (ℓs ℓs' : listset label) : *)
+(*   equiv_LabelRel (disj (unary_conj (fun ℓ => ℓ ∈ ℓs)) (unary_conj (fun ℓ => ℓ ∈ ℓs'))) *)
+(*     (unary_conj (fun ℓ => ℓ ∈ ℓs ∪ ℓs')). *)
+(* Proof. *)
+(*   intros ℓ ℓ'. split; intro H. eauto. *)
